@prefix gviz: <http://lig-tdcge.imag.fr/steamer/covikoa/geoviz#> .
@prefix ion: <http://lig-tdcge.imag.fr/steamer/covikoa/interaction#> .
@prefix owl: <http://www.w3.org/2002/07/owl#> .
@prefix rdf: <http://www.w3.org/1999/02/22-rdf-syntax-ns#> .
@prefix rdfs: <http://www.w3.org/2000/01/rdf-schema#> .
@prefix term: <http://purl.org/dc/terms/> .
@prefix vann: <http://purl.org/vocab/vann/> .
@prefix xml: <http://www.w3.org/XML/1998/namespace> .
@prefix xsd: <http://www.w3.org/2001/XMLSchema#> .
@base <http://lig-tdcge.imag.fr/steamer/covikoa/geoviz#> .


<http://lig-tdcge.imag.fr/steamer/covikoa/geoviz> a owl:Ontology ;
                                                  term:creator "Matthieu Viry" ;
                                                  term:issued "2020-09-30"^^xsd:date ;
                                                  owl:versionInfo "0.2.0" ;
                                                  term:license "http://creativecommons.org/licenses/by-nc-sa/4.0/"^^term:URI ;
                                                  vann:preferredNamespacePrefix "gviz" ;
                                                  vann:preferredNamespaceUri "http://lig-tdcge.imag.fr/steamer/covikoa/geoviz#"^^xsd:string ;
                                                  rdfs:comment """ The CoViKoa-geoviz ontology is a generic, extensible, high-level vocabulary describing what a geovisualization user interface can be."""@en .


#################################################################
#    Annotation properties
#################################################################

###  http://purl.org/dc/terms/creator
<http://purl.org/dc/terms/creator> rdf:type owl:AnnotationProperty .


###  http://purl.org/dc/terms/issued
<http://purl.org/dc/terms/issued> rdf:type owl:AnnotationProperty .


###  http://purl.org/dc/terms/license
<http://purl.org/dc/terms/license> rdf:type owl:AnnotationProperty .


###  http://purl.org/vocab/vann/preferredNamespacePrefix
<http://purl.org/vocab/vann/preferredNamespacePrefix> rdf:type owl:AnnotationProperty .


###  http://purl.org/vocab/vann/preferredNamespaceUri
<http://purl.org/vocab/vann/preferredNamespaceUri> rdf:type owl:AnnotationProperty .


#################################################################
#    Classes
#################################################################

gviz:GeoVisualApplication a owl:Class ;
                          rdfs:label "GeoVisual Application"@en, "Application de Geovisualisation"@fr ;
                          rdfs:comment "Describes a geo-visualization software application, implying the interface to view and interact with geospatial data for a given purpose."@en,
"Décrit une application logicielle de geovisualiation, sous-entendu l'interface permettant de visualiser et d'interagir avec des donnees geospatiales pour une finalité donnée."@fr .

gviz:GeoVisualIntermediateRepresentation a owl:Class ;
                             rdfs:label "GeoVisual Intermediate Representation"@en, "Representation Intermédiaire Géovisuelle"@fr ;
                             rdfs:comment "Describes a geospatial feature for which we want to obtain a portrayal for a given component."@en .

gviz:GeoVisualComponent a owl:Class ;
                        rdfs:label "GeoVisual Component"@en, "Composant Géovisuel"@fr ;
                        rdfs:comment "Describes a component aimed at geovisualisation."@en .

gviz:Map2dComponent a owl:Class ;
                    rdfs:subClassOf gviz:GeoVisualComponent ;
                    rdfs:comment """Describes a geovisual component that consists of a 2d map, such as those that can be built with OpenLayers or Leaflet for example."""@en .

gviz:Map3dComponent a owl:Class ;
                    rdfs:subClassOf gviz:GeoVisualComponent ;
                    rdfs:comment """Describes a geovisual component that consists of a 3d map, such as those that can be built with iTowns or Cesium for example."""@en .

gviz:LegendComponent a owl:Class ;
                     rdfs:subClassOf gviz:GeoVisualComponent  ;
                     rdfs:comment """Describes a legend component that can be linked to another geovisual component, typically the 2d map or the 3d map, to synchronize the information shown."""@en .

gviz:TableComponent a owl:Class ;
                    rdfs:subClassOf gviz:GeoVisualComponent ;
                    rdfs:comment """Describes a table component that can be used to display the information about the features of a gviz:Portrayal."""@en .

gviz:PopupComponent a owl:Class ;
                    rdfs:subClassOf gviz:GeoVisualComponent ;
                    rdfs:comment """Describes a popup component that can be used to display the information about a single feature, or 'compare' information between two features for example."""@en .

gviz:StaticContentComponent a owl:Class ;
                            rdfs:subClassOf gviz:GeoVisualComponent ;
                            rdfs:comment """Describes a component that displays static, pre-written HTML content (such as an insert with the project logo, etc.)."""@en .

gviz:FilterComponent a owl:Class ;
                     rdfs:subClassOf gviz:GeoVisualComponent ;
                     rdfs:comment """Describes a component that can filter the data displayed on a component to which it is linked."""@en .

gviz:Materialisation a owl:Class ;
    rdfs:label "Materialisation"@en , "Matérialisation"@fr ;
    rdfs:comment "Describes the materialisation of an individual represented (via gviz:represents) by a gviz:GeoVisualIntermediateRepresentation."@en .

gviz:Portrayal a owl:Class ;
    rdfs:subClassOf <https://gis.lu.se/ont/data_portrayal/style#Style> ;
    rdfs:label "Portrayal"@en , "Représentation"@fr ;
    rdfs:comment """This is a portrayal style necessary to build a complete portrayal, linked to one or more gviz:PortrayalRules.
     In order to add extra-semantics to this class we define it as a subClassOf style:Style (defined in Fellah, 2017 and reused in Huang & Harrie, 2020).
     """@en .

gviz:hasSymbol a owl:Class ;
               rdfs:domain gviz:PortrayalRule ;
               rdfs:range <https://gis.lu.se/ont/data_portrayal/symbol#Symbol> .

gviz:PortrayalRule a owl:Class ;
                   rdfs:label "Portrayal Rule"@en , "Règle de représentation"@fr ;
                   rdfs:comment """
                   This is a rule for linking entities to their symbolizer.
                   It is the content of this rule that allows the entities (of the concept represented by the parent gviz:Portrayal) to be specified,
                   potentially with a cvkd:PropertyConstraint and/or a cvkd:SpatialConstraint, which corresponds to the symbol linked with gviz:hasSymbol."""@fr .


<https://gis.lu.se/ont/data_portrayal/style#Style> a owl:Class .

<https://gis.lu.se/ont/data_portrayal/symbol#Symbol> a owl:Class .

<https://gis.lu.se/ont/data_portrayal/symbolizer#Symbolizer> a owl:Class .

#################################################################
#    Properties
#################################################################

<https://gis.lu.se/ont/data_portrayal/symbolizer#hasSymbolizer> a owl:ObjectProperty ;
    rdfs:domain <https://gis.lu.se/ont/data_portrayal/symbol#Symbol> ;
    rdfs:range <https://gis.lu.se/ont/data_portrayal/symbolizer#Symbolizer> .

gviz:hasGeoVisualComponent a owl:ObjectProperty ;
                           rdfs:label "has GeoVisual Component"@en, "a Composant Géovisuel"@fr ;
                           rdfs:domain gviz:GeoVisualApplication ;
                           rdfs:range gviz:GeoVisualComponent .


gviz:represents a owl:ObjectProperty ;
                rdfs:label "represents"@en, "représente"@fr ;
                rdfs:domain [ a owl:Class ;
                              owl:unionOf (gviz:GeoVisualApplication gviz:GeoVisualIntermediateRepresentation) ;
                  ] ;
                rdfs:range owl:Thing ;
                rdfs:comment """
                    This is the property which is used to link a GeoVisualIntermediateRepresentation (and optionally a gviz:GeoVisualApplication) to the corresponding
                    concept in the targeted Semantic Data Model.
                    """@en .

gviz:presentsGVR a owl:ObjectProperty  ;
                 rdfs:label "presents GeoVisualIntermediateRepresentation"@en , "présente GeoVisualIntermediateRepresentation"@fr ;
                 rdfs:domain gviz:GeoVisualComponent ;
                 rdfs:range gviz:GeoVisualIntermediateRepresentation ;
                 rdfs:comment """
                    This is the property which is used to link a GeoVisualComponent to the gviz:GeoVisualIntermediateRepresentation
                    that are depicted on him. Note that multiple GeoVisualComponents (Map2dComponent) can be linked to a GeoVisualIntermediateRepresentation when
                    the same entity appears on multiple map. See the gviz:appearsIn property to know which gviz:Materialisation have to be shown on which GeoVisualComponent."""@en .

gviz:denotesConcept a owl:ObjectProperty ;
                    rdfs:label "denotes Concept"@en , "denote Concept"@fr ;
                    rdfs:domain [ a owl:Class ;
                                  owl:unionOf (gviz:Portrayal <https://gis.lu.se/ont/data_portrayal/symbol#Symbol>) ;
                      ] ;
                    rdfs:range owl:Class ;
                    rdfs:comment """
                    This is the property which is used on a gviz:Portrayal or on symb:Symbol to link to the concept from the SDM that is denoted in the Portrayal or by the Symbol.

                    Because of the particular organization of data in RDFS/OWL, it seems necessary to specify that a particular portrayal *or* a particular symbol can denote a concept of the targeted domain. This allows us to reorganize the knowledge sometimes necessary for the creation of the geovisualization (as mentioned by Villanova-Oliver, 2018).
                    We differ in this from Fellah (2017) and Huang and Harrie (2020) and their <https://gis.lu.se/ont/data_portrayal/symbol#denotes> property.
                    """@en .

gviz:linkedTo a owl:ObjectProperty , owl:SymmetricProperty ;
              rdfs:label "linked to"@en , "lié a"@fr ;
              rdfs:domain gviz:GeoVisualComponent ;
              rdfs:range gviz:GeoVisualComponent ;
              rdfs:comment """
              Describes a link between two components.
              This is typically used to describe that a specific LegendComponent is linked to a specific 2D Map
              and benefit to the default behavior of having the legend built automatically."""@en .

gviz:hasCenterAndResolutionSynchronizedWith a owl:ObjectProperty , owl:SymmetricProperty ;
              rdfs:subPropertyOf gviz:linkedTo ;
              rdfs:label "has Center And Resolution Synchronized With"@en , "a centre et résolution synchronisés avec"@fr ;
              rdfs:domain gviz:Map2dComponent ;
              rdfs:range gviz:Map2dComponent ;
              rdfs:comment """
              Describes a synchronization link between two Map2dComponent.
              This is a special case of linking in which the view
              (center point and zoom level, not map extent - this is important if the two map dont have the same size)
              is synchronised between the two Map2dComponent.
              Domain / range may be extended to Map3dComponent in the future."""@en .

gviz:hasCenterAndExtentSynchronizedWith a owl:ObjectProperty , owl:SymmetricProperty ;
            rdfs:subPropertyOf gviz:linkedTo ;
            rdfs:label "has Center And Extent Synchronized With"@en , "a centre et étendue synchronisés avec"@fr ;
            rdfs:domain gviz:Map2dComponent ;
            rdfs:range gviz:Map2dComponent ;
            rdfs:comment """
              Describes a synchronization link between two Map2dComponent.
              This is a special case of linking in which the view
              (center point and zoom level, not map extent - this is important if the two map dont have the same size)
              is synchronised between the two Map2dComponent.
              Domain / range may be extended to Map3dComponent in the future."""@en .


gviz:hasMaterialisation rdf:type owl:ObjectProperty ;
                        rdfs:label "has materialisation"@en , "a representation"@fr ;
                        rdfs:domain gviz:GeoVisualIntermediateRepresentation ;
                        rdfs:range gviz:Materialisation .

gviz:isSymbolizedBy rdf:type owl:ObjectProperty ;
                            rdfs:label "is symbolized by"@en , "est symbolisé par"@fr ;
                            rdfs:domain gviz:Materialisation ;
                            rdfs:range <https://gis.lu.se/ont/data_portrayal/symbolizer#Symbolizer> .

gviz:appearsIn rdf:type owl:ObjectProperty ;
               rdfs:label "appears in"@en , "apparait dans"@fr ;
               rdfs:domain gviz:Materialisation ;
               rdfs:range gviz:GeoVisualComponent ;
               rdfs:comment """Describe the fact that a gviz:Materialisation appears on a specific gviz:GeoVisualComponent."""@en .

gviz:onComponent rdf:type owl:ObjectProperty ;
                 rdfs:label "on Component"@en , "sur le composant"@fr ;
                 rdfs:domain gviz:Portrayal ;
                 rdfs:range gviz:GeoVisualComponent ;
                 rdfs:comment """Describe the fact that a gviz:Portrayal is intended to appear on a specific gviz:GeoVisualComponent."""@en .

gviz:hasPortrayalRule a owl:ObjectProperty ;
                      rdfs:label "has portrayal rule"@en , "a règle de représentation"@fr ;
                      rdfs:domain gviz:Portrayal ;
                      rdfs:range gviz:PortrayalRule ;
                      rdfs:comment """Links a Portrayal to one or more PortrayalRules."""@en .

gviz:hasSymbol a owl:ObjectProperty ;
                rdfs:label "has symbol"@en , "a symbole"@fr ;
                rdfs:domain gviz:PortrayalRule ;
                rdfs:range <https://gis.lu.se/ont/data_portrayal/symbol#Symbol> .

gviz:displayIndex rdf:type owl:DatatypeProperty , owl:FunctionalProperty ;
                  rdfs:label "display index"@en , "index d'affichage"@fr ;
                  rdfs:domain [ a owl:Class ;
                                owl:unionOf (gviz:Materialisation gviz:Portrayal gviz:PortrayalRule) ;
                           ] ;
                  rdfs:range xsd:integer ;
                  rdfs:comment """
                    Describe the index on which the features portrayed by these parameters have to appear.
                    The displayIndex is defined as the inverse of the z-index, so 0 means top layer and 9999 means the lowest bottom layer."""@en .
